typeclass: fix typeclass_env_map_impl

typeclass/typeclass_env_map_implScript.sml
@@ -7,6 +7,7 @@ open mlmapTheory mlstringTheory balanced_mapTheory alistTheory topological_sortT
 open miscTheory;
 open typeclass_typesTheory typeclass_typesPropsTheory;
 open typeclass_texpTheory;
+open typeclass_typingTheory typeclass_typingPropsTheory;
 open monadsyntax;
 
 val _ = new_theory "typeclass_env_map_impl";
@@ -14,24 +15,36 @@ val _ = new_theory "typeclass_env_map_impl";
 val _ = monadsyntax.enable_monadsyntax()
 val _ = monadsyntax.enable_monad "option"
 
+
+(* Since we only support single-param typeclass, we only need to keep
+* track of the names of the super classes *)
 Datatype:
   classinfo_impl =
-    <| super : mlstring list
+    <| supers : mlstring list
      ; kind : Kind option
-     ; methodsig : (cvname, PredType) mlmap$map
-     ; minImp : minImplAST
-     ; defaults : (cvname, texp) mlmap$map |>
+     ; methodsig : (cvname, 'a # PredType) mlmap$map
+     ; defaults : (cvname, 'a texp) mlmap$map |>
 End
 
+(* We only support the form where there is only one constructor on the
+* right, and every constraint in the context can only refer to a type
+* variabale *)
 Datatype:
   instinfo_impl =
-    <| cstr : (mlstring # num) list (* class and type variable *)
-     ; nargs : num (* number of arguments to the type constructor *)
-     ; impl : (cvname, texp) mlmap$map |> (* function name and its expression *)
+    <| cstr : (mlstring # num) list (* list of classes and type vars *)
+     ; impls : (cvname, 'a texp) mlmap$map |>
+     (* method name and its implementation *)
 End
 
-Type class_map_impl = ``:(mlstring, classinfo_impl) map``;
-Type inst_map_impl = ``:((mlstring # ty_cons), instinfo_impl) map``;
+(* class name to class info *)
+Type class_map_impl = ``:(mlstring, 'a classinfo_impl) map``;
+
+(* NOTE: We don't actually need to record the number of
+ * type arguments as it can be inferred from the
+ * kind, but it should make things simpler *)
+(* class name, the constructor and
+* the number of type arguments to instance info *)
+Type inst_map_impl = ``:((mlstring # ty_cons # num), 'a instinfo_impl) map``;
 
 Definition built_in_ty_num_def:
   built_in_ty_num (PrimT Bool) = 0 ∧
@@ -80,6 +93,7 @@ Definition inst_map_cmp_def:
   inst_map_cmp = mlstring$compare lexTO ty_consOrd
 End
 
+(* The ordering for instance map *)
 Theorem TO_inst_map_cmp:
   TotOrd inst_map_cmp
 Proof
@@ -108,145 +122,174 @@ Proof
   simp[cmp_of_empty,init_inst_map_def]
 QED
 
-Definition to_class_map_def:
-  to_class_map (m:class_map_impl) = FMAP_MAP2 (λ(k,x).
-    <| super := x.super
-     ; kind := x.kind
-     ; methodsig := to_fmap x.methodsig
-     ; minImp := x.minImp
-     ; defaults := to_fmap x.defaults |>) (to_fmap m)
+Definition class_super_abs_rel_def:
+  class_super_abs_rel (cl_impl: 'a classinfo_impl) (abs:Class) =
+    (set (cl_impl.supers) = set (MAP FST abs.supers))
 End
 
-Definition to_inst_map_def:
-  to_inst_map (m:inst_map_impl) =
-    FMAP_MAP2 (λ(k,inf).
-      <|cstr := inf.cstr
-       ;nargs := inf.nargs
-       ;impl := to_fmap inf.impl|>)
-    (to_fmap m)
+(* relating the concrete class and its abstraction *)
+Definition class_abs_rel_def:
+  class_abs_rel (cl_impl:Kind list classinfo_impl) (abs:Class) =
+    (class_super_abs_rel cl_impl abs ∧
+    cl_impl.kind = SOME abs.kind ∧
+    lookup cl_impl.methodsig = ALOOKUP abs.methods)
 End
 
-Theorem FLOOKUP_to_class_map:
-  map_ok cl_map ⇒
-    (FLOOKUP (to_class_map cl_map) c = SOME x ⇔
-    ∃y. lookup cl_map c = SOME y ∧
-      x = <| super := y.super
-           ; kind := y.kind
-           ; methodsig := to_fmap y.methodsig
-           ; minImp := y.minImp
-           ; defaults := to_fmap y.defaults |>)
+(* relating the class map and its abstraction *)
+Definition class_map_abs_rel_def:
+  class_map_abs_rel (cl_map_impl:Kind list class_map_impl) (abs:class_map) =
+  (∀c. OPTREL class_abs_rel (mlmap$lookup cl_map_impl c) (ALOOKUP abs c))
+End
+
+Definition class_map_super_abs_rel_def:
+  class_map_super_abs_rel (cl_map_impl: 'a class_map_impl) (abs:class_map) =
+  (∀c. OPTREL class_super_abs_rel (lookup cl_map_impl c) (ALOOKUP abs c))
+End
+
+Theorem class_map_abs_rel_IMP_class_map_super_abs_rel:
+  class_map_abs_rel cl_map_impl abs ⇒
+  class_map_super_abs_rel cl_map_impl abs
 Proof
-  rw[to_class_map_def,FLOOKUP_FMAP_MAP2,FMAP_MAP2_THM,
-    GSYM mlmapTheory.lookup_thm]
+  rw[class_map_abs_rel_def,class_map_super_abs_rel_def] >>
+  last_x_assum $ qspec_then `c` assume_tac >>
+  drule_at_then (Pos last) irule OPTREL_MONO >>
+  simp[class_abs_rel_def]
 QED
 
+(* every class in the super list must be a valid key of the map *)
+Definition super_keys_ok_def:
+  super_keys_ok (cl_map: 'a class_map_impl) =
+  (∀c clinfo c'.
+    mlmap$lookup cl_map c = SOME clinfo ∧ MEM c' clinfo.supers ⇒
+    ∃x. mlmap$lookup cl_map c' = SOME x)
+End
+
+(* relating a concrete instance with its abstraction *)
+Definition inst_abs_rel_def:
+  inst_abs_rel class tycons ntargs (inst_impl:Kind list instinfo_impl)
+    (abs:Kind list Instance) =
+  (abs.context = MAP (λ(cl,v). (cl,TypeVar v)) inst_impl.cstr ∧
+   ALOOKUP abs.impls = lookup inst_impl.impls ∧
+   abs.class = class ∧
+   abs.type = tcons_to_type tycons (GENLIST TypeVar ntargs) ∧
+   LENGTH abs.kinds = ntargs)
+End
+
+(* relating a concrete instance map with its abstraction *)
+Definition inst_map_abs_rel_def:
+  inst_map_abs_rel
+    (inst_map_impl:Kind list inst_map_impl)
+    (abs_map:Kind list instance_list) ⇔
+  (∀cl tycons ntargs instinfo.
+    lookup inst_map_impl (cl,tycons,ntargs) = SOME instinfo ⇒
+      ∃abs. MEM abs abs_map ∧
+        inst_abs_rel cl tycons ntargs instinfo abs) ∧
+  (∀abs. MEM abs abs_map ⇒
+    ∃cl tycons ntargs instinfo.
+      lookup inst_map_impl (cl,tycons,ntargs) = SOME instinfo ∧
+      inst_abs_rel cl tycons ntargs instinfo abs)
+End
+
+(* return NONE if duplicated *)
 Definition add_instance_def:
-  add_instance (inst_map:inst_map_impl) cl ty info =
+  add_instance (inst_map:'a inst_map_impl) cl ty info =
     case lookup inst_map (cl,ty) of
     | NONE => SOME $ insert inst_map (cl,ty) info
     | SOME _ => NONE
 End
 
-(* check if there is cyclic superclass relation *)
+(* `super_reachable_abs cl_map c s`
+* checks if `s` is a parent of the class `c` *)
+Definition super_reachable_abs_def:
+  super_reachable_abs (cl_map: class_map) =
+  TC (λclname supername.
+    ∃cl. ALOOKUP cl_map clname = SOME cl ∧
+      MEM supername (MAP FST cl.supers))
+End
+
+(* implementation of super_reachable_abs *)
+Definition super_reachable_def:
+  super_reachable (cl_map:'a class_map_impl) =
+  TC (λclname supername.
+    ∃cl. lookup cl_map clname = SOME cl ∧ MEM supername cl.supers)
+End
+
+(* RTC version of super_reachable *)
+Definition super_reachable_RTC_def:
+  super_reachable_RTC (cl_map:'a class_map_impl) =
+  RTC (λclname supername.
+    ∃cl. lookup cl_map clname = SOME cl ∧ MEM supername cl.supers)
+End
+
+Theorem super_reachable_RTC_CASES_super_reachable:
+  super_reachable_RTC cl_map c s =
+  (c = s ∨ super_reachable cl_map c s)
+Proof
+  simp[super_reachable_RTC_def,super_reachable_def,
+    RTC_CASES_TC]
+QED
+
+Theorem class_map_super_abs_rel_super_reachable:
+  class_map_super_abs_rel cl_map_impl cl_map ⇒
+  super_reachable cl_map_impl = super_reachable_abs cl_map
+Proof
+  rw[class_map_super_abs_rel_def,super_reachable_def,
+    super_reachable_abs_def] >>
+  AP_TERM_TAC >>
+  rw[FUN_EQ_THM] >>
+  first_x_assum $ qspec_then `clname` mp_tac >>
+  rw[OPTREL_def] >>
+  gvs[class_super_abs_rel_def]
+QED
+
+Definition super_no_cycles_abs_def:
+  super_no_cycles_abs cl_map =
+    ∀clname. ¬super_reachable_abs cl_map clname clname
+End
+
+Definition super_no_cycles_def:
+  super_no_cycles cl_map = ∀clname. ¬super_reachable cl_map clname clname
+End
+
+Theorem class_map_super_abs_rel_super_no_cycles:
+  class_map_super_abs_rel cl_map_impl cl_map ⇒
+  super_no_cycles cl_map_impl = super_no_cycles_abs cl_map
+Proof
+  rw[super_no_cycles_def,super_no_cycles_abs_def] >>
+  drule class_map_super_abs_rel_super_reachable >>
+  simp[]
+QED
+
 Definition superAList_def:
   superAList cl_map =
-    MAP (λ(k,v). (k, v.super)) $ toAscList cl_map
+    MAP (λ(k,v). (k, v.supers)) $ toAscList cl_map
 End
 
-Definition check_cl_map_no_cycles_def:
-  check_cl_map_no_cycles cl_map =
-    ¬has_cycle (superAList cl_map)
-End
-
-Theorem fmap_to_alist_MAP_KEYS:
-  INJ f (FDOM m) UNIV ⇒
-  set (fmap_to_alist (MAP_KEYS f m)) =
-    set (MAP (λ(k,v). (f k,v)) $ fmap_to_alist m)
-Proof
-  Induct_on `m` >>
-  rw[] >>
-  `INJ f (FDOM m) UNIV`
-  by (
-    drule_then irule INJ_SUBSET >>
-    simp[]
-  ) >>
-  drule_then (fn t => simp[t]) MAP_KEYS_FUPDATE >>
-  fs[EXTENSION,LAMBDA_PROD,GSYM PFORALL_THM] >>
-  rpt gen_tac >>
-  simp[MEM_MAP,MEM_fmap_to_alist,
-    LAMBDA_PROD,GSYM PEXISTS_THM,FLOOKUP_UPDATE] >>
-  iff_tac
-  >- (
-    IF_CASES_TAC
-    >- (
-      rw[] >>
-      irule_at (Pos hd) EQ_REFL >>
-      simp[]) >>
-    rw[MEM_MAP] >>
-    pairarg_tac >>
-    fs[] >>
-    irule_at (Pos hd) EQ_REFL >>
-    fs[FDOM_FLOOKUP,FAPPLY_FUPDATE_THM] >>
-    IF_CASES_TAC >>
-    fs[FLOOKUP_DEF]) >>
-  fs[MEM_MAP,FAPPLY_FUPDATE_THM,LAMBDA_PROD,
-    GSYM PEXISTS_THM] >>
-  rw[]
-  >- (
-    IF_CASES_TAC >>
-    fs[INJ_DEF] >>
-    spose_not_then kall_tac >>
-    pop_assum mp_tac >>
-    simp[]) >>
-  irule_at (Pos hd) EQ_REFL >>
-  IF_CASES_TAC >>
-  fs[FLOOKUP_DEF]
-QED
-
-Triviality set_MAP_SINGLE_FST_EQ:
-  (∀x y. f x = f y ⇔ x = y) ∧
-  set (MAP f x) = set (MAP f y) ⇒
-  set x = set y
-Proof
-  simp[LIST_TO_SET_MAP] >>
-  metis_tac[IMAGE_11]
-QED
-
-Triviality set_MAP_key_EQ:
-  set (MAP (λ(k,v). ({k},v)) x) = set (MAP (λ(k,v). ({k},v)) y) ⇒
-  set x = set y
-Proof
-  qpat_abbrev_tac `f=(λ(k,v). ({k},v))` >>
-  strip_tac >>
-  drule_at_then (Pos last) irule set_MAP_SINGLE_FST_EQ >>
-  rw[Abbr`f`,EQ_IMP_THM] >>
-  ntac 2 (pairarg_tac >> fs[])
-QED
-
-Theorem mlmap_toAscList:
-  map_ok (m:('a,'b) map) ⇒
-  SORTED (λ(x,y) (x',y'). (cmp_of m) x x' = Less) (toAscList m) ∧
-  (set (toAscList m)) =
-    set (fmap_to_alist (
-      (to_fmap: ('a,'b) map -> ('a |-> 'b)) m))
+Theorem mlmap_ALOOKUP_toAscList:
+  map_ok m ⇒
+  ALOOKUP (mlmap$toAscList m) = mlmap$lookup m
 Proof
   Cases_on `m` >>
-  simp[map_ok_def,mlmapTheory.toAscList_def,cmp_of_def] >>
-  strip_tac >>
-  drule_then assume_tac comparisonTheory.TotOrder_imp_good_cmp >>
-  drule_all balanced_mapTheory.toAscList_thm >>
-  rw[] >>
-  drule_then assume_tac to_fmap_thm >>
-  drule_then assume_tac TotOrd_key_set >>
-  fs[lift_key_def,GSYM LIST_TO_SET_MAP,MAP_KEYS_def] >>
-  irule set_MAP_key_EQ >>
-  qmatch_goalsub_abbrev_tac `MAP _ (fmap_to_alist m)` >>
-  `INJ (λx. {x}) (FDOM m) UNIV` by simp[INJ_DEF] >>
-  drule fmap_to_alist_MAP_KEYS >>
-  rw[]
+  rw[FUN_EQ_THM,mlmapTheory.toAscList_def,map_ok_def,
+    mlmapTheory.lookup_def] >>
+  irule ALOOKUP_toAscList >>
+  simp[] >>
+  drule_then (irule_at Any) comparisonTheory.TotOrder_imp_good_cmp >>
+  gvs[totoTheory.TotOrd]
 QED
 
-Triviality ALL_DISTINCT_superAList:
+Theorem super_reachable_TC_depends_on_weak:
+  map_ok cl_map ⇒
+  super_reachable cl_map = TC_depends_on_weak (superAList cl_map)
+Proof
+  simp[TC_depends_on_weak_def,super_reachable_def,superAList_def,
+    ALOOKUP_MAP,PULL_EXISTS] >>
+  strip_tac >>
+  AP_TERM_TAC >>
+  rw[FUN_EQ_THM,mlmap_ALOOKUP_toAscList]
+QED
+
+Theorem ALL_DISTINCT_superAList:
   map_ok cl_map ⇒
   ALL_DISTINCT (MAP FST $ superAList cl_map)
 Proof
@@ -254,42 +297,22 @@ Proof
   simp[mlmapTheory.MAP_FST_toAscList]
 QED
 
-Triviality super_reachable_EQ_TC_depends_on_weak:
-  map_ok cl_map ⇒
-  super_reachable (to_class_map cl_map) =
-    TC_depends_on_weak (superAList cl_map)
-Proof
-  rw[super_reachable_def,TC_depends_on_weak_def] >>
-  AP_TERM_TAC >>
-  rw[FUN_EQ_THM,superAList_def,map_fst,depends_on1_def] >>
-  fs[to_class_map_def,FLOOKUP_FMAP_MAP2,FMAP_MAP2_THM,PULL_EXISTS] >>
-  drule_then strip_assume_tac mlmap_toAscList >>
-  gvs[ALOOKUP_MAP,PULL_EXISTS,EXTENSION] >>
-  rw[EQ_IMP_THM]
-  >- (
-    drule_then assume_tac $
-      cj 2 mlmapTheory.MAP_FST_toAscList >>
-    drule_then assume_tac ALOOKUP_ALL_DISTINCT_MEM >>
-    drule_then strip_assume_tac mlmap_toAscList >>
-    fs[EXTENSION] >>
-    metis_tac[]
-  ) >>
-  drule_then assume_tac ALOOKUP_MEM >>
-  drule_then assume_tac $ cj 2 mlmap_toAscList >>
-  fs[EXTENSION]
-QED
+(* algorithm for checking acyclic superclass relation *)
+Definition check_cl_map_no_cycles_def:
+  check_cl_map_no_cycles cl_map =
+    ¬has_cycle (superAList cl_map)
+End
 
 Theorem check_cl_map_no_cycles_IMP_super_no_cycles:
   map_ok cl_map ∧
   check_cl_map_no_cycles cl_map ⇒
-  super_no_cycles $ to_class_map cl_map
+  super_no_cycles cl_map
 Proof
-  rw[super_no_cycles_def] >>
-  drule_all_then assume_tac
-    super_reachable_EQ_TC_depends_on_weak >>
+  rw[super_no_cycles_def,super_reachable_TC_depends_on_weak] >>
   drule_then assume_tac ALL_DISTINCT_superAList >>
-  drule_then assume_tac has_cycle_correct2 >>
-  fs[check_cl_map_no_cycles_def]
+  strip_tac >>
+  drule_then drule $ SRULE[PULL_EXISTS] $ iffRL has_cycle_correct2 >>
+  gvs[check_cl_map_no_cycles_def]
 QED
 
 (* Similar to how it is implemented in
@@ -302,9 +325,9 @@ Proof
   simp[mlmapTheory.lookup_thm,flookup_thm]
 QED
 
-Triviality super_reachable_FDOM_cl_map:
-  ∀c s. super_reachable m c s ⇒
-  ∃x i. FLOOKUP m x = SOME i ∧ MEM s i.super
+Theorem super_reachable_FDOM_cl_map:
+  ∀c s. super_reachable cl_map c s ⇒
+  ∃x cl. lookup cl_map x = SOME cl ∧ MEM s cl.supers
 Proof
   simp[super_reachable_def] >>
   ho_match_mp_tac TC_INDUCT >>
@@ -314,75 +337,62 @@ QED
 
 Theorem super_reachable_FINITE:
   map_ok cl_map ⇒
-  FINITE {s | super_reachable (to_class_map cl_map) c s}
+  FINITE (super_reachable cl_map c)
 Proof
   rw[] >>
   irule SUBSET_FINITE >>
-  qexists `BIGUNION (IMAGE (\info. set info.super) $
-      {info | ?c. FLOOKUP (to_class_map cl_map) c = SOME info})` >>
-  simp[] >>
-  irule_at (Pos hd) IMAGE_FINITE >>
-  rw[]
-  >- (
-    simp[super_reachable_def,to_class_map_def,
-      FMAP_MAP2_THM,FLOOKUP_FMAP_MAP2,PULL_EXISTS] >>
-    qmatch_goalsub_abbrev_tac `FINITE m` >>
-    `m = IMAGE (\c. let v = to_fmap cl_map ' c in
-        <|super := v.super; kind := v.kind;
-          methodsig := to_fmap v.methodsig;
-          minImp := v.minImp;
-          defaults := to_fmap v.defaults|>)
-         {c | ∃v. (FLOOKUP (to_fmap cl_map) c = SOME v)}`
-      by (
-        simp[Abbr`m`,IMAGE_DEF,EXTENSION,flookup_thm] >>
-        metis_tac[]
-      ) >>
-     simp[] >>
-     irule IMAGE_FINITE >>
-     simp[flookup_thm]) >>
-  rw[SUBSET_DEF] >>
+  qexists `BIGUNION (IMAGE (λcl. set cl.supers) $
+    {v | ∃s. mlmap$lookup cl_map s = SOME v})` >>
+  rw[SUBSET_DEF]
+  >- (  
+    irule IMAGE_FINITE >>
+    simp[mlmapTheory.lookup_thm,GSYM TO_FLOOKUP]
+  )
+  >- simp[] >>
+  gvs[IN_DEF] >>
   drule super_reachable_FDOM_cl_map >>
   rw[] >>
-  metis_tac[SUBSET_DEF]
+  first_assum $ irule_at (Pos last) >>
+  gvs[IN_DEF]
+QED
+
+Triviality GSPEC_super_reachable_or:
+  {s | super_reachable cl_map c s ∨ c = s} =
+    super_reachable cl_map c ∪ {c}
+Proof
+  rw[EXTENSION] >>
+  metis_tac[IN_DEF]
 QED
 
 Theorem super_reachable_list_FINITE:
   map_ok cl_map ⇒
   FINITE {s | ∃c. MEM c cs ∧
-    (super_reachable (to_class_map cl_map) c s ∨
-      c = s)}
+    (super_reachable cl_map c s ∨ c = s)}
 Proof
   strip_tac >>
   qmatch_goalsub_abbrev_tac `FINITE X` >>
-  `X = BIGUNION (set $ (MAP (λc. {s | super_reachable (to_class_map cl_map) c s ∨ c =
+  `X = BIGUNION (set $ (MAP (λc. {s | super_reachable cl_map c s ∨ c =
   s}) cs))`
-    by (
-      simp[Abbr`X`,BIGUNION,MEM_MAP,EXTENSION] >>
-      rw[EQ_IMP_THM,PULL_EXISTS]
-      >- (
-        qexists_tac `\x. super_reachable (to_class_map cl_map) c x ∨ c = x` >>
-        simp[IN_DEF] >>
-        qexists_tac`c` >>
-        fs[SUBSET_DEF,IN_DEF]
-      )
-      >- (
-        qexists_tac `\x. super_reachable (to_class_map cl_map) c x ∨ c = x` >>
-        simp[IN_DEF] >>
-        qexists_tac`c` >>
-        fs[SUBSET_DEF,IN_DEF]
-      ) >>
-      metis_tac[]
+  by (
+    simp[Abbr`X`,BIGUNION,MEM_MAP,EXTENSION] >>
+    rw[EQ_IMP_THM,PULL_EXISTS]
+    >- (
+      qexists_tac `\x. super_reachable cl_map c x ∨ c = x` >>
+      simp[IN_DEF] >>
+      qexists_tac`c` >>
+      fs[SUBSET_DEF,IN_DEF]
+    )
+    >- (
+      qexists_tac `\x. super_reachable cl_map c x ∨ c = x` >>
+      simp[IN_DEF] >>
+      qexists_tac`c` >>
+      fs[SUBSET_DEF,IN_DEF]
     ) >>
-    rw[MEM_MAP] >>
-    `{s | super_reachable (to_class_map cl_map) c s ∨ c = s} =
-    {s | super_reachable (to_class_map cl_map) c s} ∪ {c}`
-      by (
-        rw[EXTENSION] >>
-        metis_tac[]
-      ) >>
-    pop_assum SUBST_ALL_TAC >>
-    simp[] >>
-    metis_tac[super_reachable_FINITE]
+    metis_tac[]
+  ) >>
+  rw[MEM_MAP,GSPEC_super_reachable_or] >>
+  simp[] >>
+  metis_tac[super_reachable_FINITE]
 QED
 
 Triviality INTER_PRESERVE_SUBSET:
@@ -413,7 +423,7 @@ Definition by_super_aux_def:
       case mlmap$lookup cl_map c of
       | NONE => NONE
       | SOME clinfo =>
-          by_super_aux_list cl_map (insert visited c t) clinfo.super t
+          by_super_aux_list cl_map (insert visited c t) clinfo.supers t
    else NONE) ∧
   by_super_aux_list cl_map ret [] t = SOME ret ∧
   by_super_aux_list cl_map visited (sup::xs) t =
@@ -427,10 +437,10 @@ Termination
   WF_REL_TAC `inv_image ($< LEX $<) (\x.
     ((case x of
     | INR (cl_map,(visited:(mlstring,'a)map),cs,t:'a) =>
-      CARD ({s | ∃c. MEM c cs ∧ (super_reachable (to_class_map cl_map) c s ∨ c = s)}
+      CARD ({s | ∃c. MEM c cs ∧ (super_reachable cl_map c s ∨ c = s)}
         DIFF {s | ∃v.  lookup visited s = SOME v})
     | INL (cl_map,visited,c,t) =>
-       CARD ({s | super_reachable (to_class_map cl_map) c s ∨ c = s}
+       CARD ({s | super_reachable cl_map c s ∨ c = s}
         DIFF {s | ∃v. lookup visited s = SOME v})),
     (case x of
     | INR (cl_map,visited,cs,t) => LENGTH cs
@@ -441,22 +451,13 @@ Termination
     conj_tac
     >- (
       irule FINITE_DIFF >>
-      drule super_reachable_FINITE >>
-      disch_then $ qspec_then `c` assume_tac >>
-      qmatch_asmsub_abbrev_tac `FINITE s` >>
-      qmatch_goalsub_abbrev_tac `FINITE s'` >>
-      `s' = s ∪ {c}`
-      by (
-        simp[Abbr`s`,Abbr`s'`,EXTENSION] >>
-        metis_tac[]
-      ) >>
-      simp[]
+      simp[GSPEC_super_reachable_or] >>
+      drule_then irule super_reachable_FINITE
     ) >>
     rw[PSUBSET_MEMBER,SUBSET_DEF,DIFF_DEF,
       mlmapTheory.lookup_insert,AllCaseEqs()]
     >- (
-      fs[super_reachable_def,to_class_map_def,
-        FMAP_MAP2_THM,FLOOKUP_FMAP_MAP2,PULL_EXISTS] >>
+      fs[super_reachable_def] >>
       disj1_tac >>
       irule TC_LEFT1_I >>
       first_assum $ irule_at (Pos last) >>
@@ -464,8 +465,7 @@ Termination
     )
     >- (Cases_on `c=x` >> fs[])
     >- (
-      fs[super_reachable_def,to_class_map_def,
-        FMAP_MAP2_THM,FLOOKUP_FMAP_MAP2,PULL_EXISTS] >>
+      fs[super_reachable_def] >>
       Cases_on `c=c'` >>
       fs[GSYM mlmapTheory.lookup_thm] >>
       irule $ cj 1 TC_RULES >>
@@ -483,14 +483,16 @@ Termination
       irule FINITE_DIFF >>
       drule_then (qspec_then `sup'::xs` assume_tac)
         super_reachable_list_FINITE >>
-      fs[]) >>
+      fs[]
+    ) >>
     PURE_REWRITE_TAC[DIFF_INTER_COMPL] >>
     irule INTER_PRESERVE_SUBSET >>
     conj_tac
     >- (
       rw[SUBSET_DEF] >>
       qexists_tac `c` >>
-      simp[]) >>
+      simp[]
+    ) >>
     irule COMPL_SUBSET >>
     simp[SUBSET_DEF,PULL_EXISTS] >>
     simp[fix_visited_def] >>
@@ -505,30 +507,28 @@ Termination
     irule FINITE_DIFF >>
     drule_then (qspec_then `sup'::xs` assume_tac)
       super_reachable_list_FINITE >>
-    fs[]) >>
+    fs[]
+  ) >>
   PURE_REWRITE_TAC[DIFF_INTER_COMPL] >>
   irule INTER_PRESERVE_SUBSET >>
   simp[SUBSET_DEF] >> metis_tac[]
 End
 
 Theorem by_super_aux_monotone:
-  (∀cl_map visited c (t:'a) new_visited.
+  (∀(cl_map:'b class_map_impl) visited c (t:'a) new_visited.
     map_ok visited ∧
     by_super_aux cl_map visited c t = SOME new_visited ⇒
       map_ok new_visited ∧
     (∀c' t. lookup visited c' = SOME t ⇒
       lookup new_visited c' = SOME t)) ∧
 
-  (∀cl_map visited cs (t:'a) new_visited.
+  (∀(cl_map:'b class_map_impl) visited cs (t:'a) new_visited.
     map_ok visited ∧
     by_super_aux_list cl_map visited cs t = SOME new_visited ⇒
       map_ok new_visited ∧
     (∀c' t. lookup visited c' = SOME t ⇒
         lookup new_visited c' = SOME t))
 Proof
-  PURE_REWRITE_TAC[super_reachable_def] >>
-  simp[to_class_map_def,FLOOKUP_FMAP_MAP2,FMAP_MAP2_THM,
-    PULL_EXISTS,GSYM $ mlmapTheory.lookup_thm] >>
   ho_match_mp_tac by_super_aux_ind >>
   reverse $ rpt conj_tac >>
   rpt gen_tac >> rpt $ disch_then strip_assume_tac >>
@@ -581,9 +581,9 @@ Theorem full_by_super_aux_ind:
   ∀P0 P1.
   (∀cl_map visited c t.
      (∀clinfo.
-         map_ok cl_map ∧ map_ok visited ∧ lookup visited c = NONE ∧
-         lookup cl_map c = SOME clinfo ⇒
-         P1 cl_map (insert visited c t) clinfo.super t) ⇒
+         map_ok cl_map ∧ map_ok visited ∧ mlmap$lookup visited c = NONE ∧
+         mlmap$lookup cl_map c = SOME clinfo ⇒
+         P1 cl_map (insert visited c t) clinfo.supers t) ⇒
       P0 cl_map visited c t) ∧
   (∀cl_map ret t. P1 cl_map ret [] t) ∧
   (∀cl_map visited sup xs t.
@@ -593,8 +593,8 @@ Theorem full_by_super_aux_ind:
        P1 cl_map visited' xs t) ∧
     (map_ok cl_map ∧ map_ok visited ⇒ P0 cl_map visited sup t) ⇒
      P1 cl_map visited (sup::xs) t) ⇒
-  (∀v0 v1 v2 v3. P0 v0 v1 v2 v3) ∧
-   ∀v0 v1 v2 v3. P1 v0 v1 v2 v3
+  (∀(v0:'b class_map_impl) v1 v2 (v3:'a). P0 v0 v1 v2 v3) ∧
+   ∀(v0:'b class_map_impl) v1 v2 (v3:'a). P1 v0 v1 v2 v3
 Proof
   rpt gen_tac >>
   strip_tac >>
@@ -604,13 +604,13 @@ Proof
 QED
 
 Theorem by_super_aux_lookup_preserve_type:
-  (∀cl_map visited c (t:'a) new_visited.
+  (∀(cl_map:'b class_map_impl) visited c (t:'a) new_visited.
   map_ok visited ∧
   by_super_aux cl_map visited c t = SOME new_visited ∧
   (∀c' v. lookup visited c' = SOME v ⇒ v = t) ⇒
   (∀c v. lookup new_visited c = SOME v ⇒ v = t)) ∧
 
-  (∀cl_map visited cs (t:'a) new_visited.
+  (∀(cl_map:'b class_map_impl) visited cs (t:'a) new_visited.
   map_ok visited ∧
   by_super_aux_list cl_map visited cs t = SOME new_visited ∧
   (∀c' v. lookup visited c' = SOME v ⇒ v = t) ⇒
@@ -653,13 +653,11 @@ Proof
 QED
 
 Theorem by_super_aux_visited:
-  (∀cl_map visited c (t:'a) new_visited.
-    by_super_aux cl_map visited c t = SOME new_visited ∧
-    map_ok visited ⇒
+  (∀(cl_map:'b class_map_impl) visited c (t:'a) new_visited.
+    by_super_aux cl_map visited c t = SOME new_visited  ⇒
     ∃v. lookup new_visited c = SOME v) ∧
-  (∀cl_map visited cs (t:'a) new_visited c.
+  (∀(cl_map:'b class_map_impl) visited cs (t:'a) new_visited c.
     by_super_aux_list cl_map visited cs t = SOME new_visited ∧
-    map_ok visited ∧
     MEM c cs ⇒
     ∃v. lookup new_visited c = SOME v)
 Proof
@@ -686,23 +684,23 @@ Proof
 QED
 
 Theorem by_super_aux_IMP_reachable:
-  (∀cl_map visited c (t:'a) new_visited.
+  (∀(cl_map:'b class_map_impl) visited c (t:'a) new_visited.
     map_ok visited ∧
     by_super_aux cl_map visited c t = SOME new_visited ⇒
     (∀c' v. lookup new_visited c' = SOME v ⇒
       RTC
-        (λsrc dst. ∃v. FLOOKUP (to_fmap cl_map) src = SOME v ∧
-        MEM dst v.super ∧ lookup visited dst = NONE) c c' ∨
+        (λsrc dst. ∃v. lookup cl_map src = SOME v ∧
+        MEM dst v.supers ∧ lookup visited dst = NONE) c c' ∨
       lookup visited c' = SOME v)) ∧
 
-  (∀cl_map visited cs (t:'a) new_visited.
+  (∀(cl_map:'b class_map_impl) visited cs (t:'a) new_visited.
     map_ok visited ∧
     by_super_aux_list cl_map visited cs t = SOME new_visited ⇒
     (∀c' v. lookup new_visited c' = SOME v ⇒
       (∃c. MEM c cs ∧ lookup visited c = NONE ∧
         RTC
-          (λsrc dst. ∃v. FLOOKUP (to_fmap cl_map) src = SOME v ∧
-          MEM dst v.super ∧ lookup visited dst = NONE) c c') ∨
+          (λsrc dst. ∃v. lookup cl_map src = SOME v ∧
+          MEM dst v.supers ∧ lookup visited dst = NONE) c c') ∨
        lookup visited c' = SOME v))
 Proof
   ho_match_mp_tac full_by_super_aux_ind >>
@@ -725,14 +723,13 @@ Proof
       Cases_on `c = c'` >- simp[] >>
       rw[]
       >- (
-        gvs[GSYM mlmapTheory.lookup_thm,
-          mlmapTheory.lookup_insert,AllCaseEqs()] >>
+        gvs[mlmapTheory.lookup_insert,AllCaseEqs()] >>
         disj1_tac >>
         irule $ cj 2 RTC_RULES >>
         qexists `c''` >>
-        fs[GSYM mlmapTheory.lookup_thm] >>
+        fs[] >>
         drule_at_then (Pos last) irule RTC_MONOTONE >>
-        rw[GSYM mlmapTheory.lookup_thm,mlmapTheory.lookup_insert] >>
+        rw[mlmapTheory.lookup_insert] >>
         fs[]
       )
       >- (
@@ -751,7 +748,7 @@ Proof
       mp_tac o SRULE[Once full_by_super_aux_def] >>
     rw[AllCaseEqs()] >>
     `map_ok visited'` by metis_tac[by_super_aux_monotone] >>
-    gvs[GSYM mlmapTheory.lookup_thm] >>
+    gvs[] >>
     reverse $ Cases_on `lookup visited c'`
     >- (
       disj2_tac >>
@@ -767,7 +764,7 @@ Proof
       rw[AllCaseEqs()] >>
       last_x_assum drule >>
       rw[] >>
-      qexists `c'''` >>
+      qexists `c''` >>
       simp[]
     ) >>
     reverse $ Cases_on `lookup visited' c'`
@@ -779,7 +776,7 @@ Proof
     ) >>
     last_x_assum drule >>
     rw[] >>
-    qexists `c'''` >>
+    qexists `c''` >>
     simp[] >>
     conj_tac
     >- metis_tac[option_CASES,by_super_aux_monotone] >>
@@ -856,21 +853,21 @@ Proof
 QED
 
 Theorem super_reachable_IMP_by_super_aux:
-  (∀cl_map visited c (t:'a) new_visited s.
+  (∀(cl_map:'b class_map_impl) visited c (t:'a) new_visited s.
     map_ok visited ∧
     by_super_aux cl_map visited c t = SOME new_visited ∧
     lookup visited c = NONE ∧
-    RTC (λsrc dst. ∃v. FLOOKUP (to_fmap cl_map) src = SOME v ∧
-      MEM dst v.super ∧ lookup visited dst = NONE) c s ⇒
-    ∃v. lookup new_visited s = SOME v) ∧
+    RTC (λsrc dst. ∃v. mlmap$lookup cl_map src = SOME v ∧
+      MEM dst v.supers ∧ mlmap$lookup visited dst = NONE) c s ⇒
+    ∃v. mlmap$lookup new_visited s = SOME v) ∧
 
-  (∀cl_map visited cs (t:'a) new_visited c s.
+  (∀(cl_map:'b class_map_impl) visited cs (t:'a) new_visited c s.
     map_ok visited ∧
     by_super_aux_list cl_map visited cs t = SOME new_visited ∧
     MEM c cs ∧ lookup visited c = NONE ∧
-    RTC (λsrc dst. ∃v. FLOOKUP (to_fmap cl_map) src = SOME v ∧
-      MEM dst v.super ∧ lookup visited dst = NONE) c s ⇒
-    ∃v. lookup new_visited s = SOME v)
+    RTC (λsrc dst. ∃v. mlmap$lookup cl_map src = SOME v ∧
+      MEM dst v.supers ∧ mlmap$lookup visited dst = NONE) c s ⇒
+    ∃v. mlmap$lookup new_visited s = SOME v)
 Proof
   ho_match_mp_tac full_by_super_aux_ind >>
   rpt conj_tac >>
@@ -898,7 +895,7 @@ Proof
     rw[mlmapTheory.lookup_insert]
     >- (
       first_x_assum $ qspec_then `0` mp_tac >>
-      simp[GSYM mlmapTheory.lookup_thm]
+      simp[]
     )
     >- (
       fs[EL_ALL_DISTINCT_EL_EQ] >>
@@ -936,7 +933,7 @@ Proof
   Cases_on `lookup visited c`
   >- (
     `map_ok visited'` by metis_tac[cj 1 by_super_aux_monotone] >>
-    gvs[PULL_EXISTS,GSYM mlmapTheory.lookup_thm] >>
+    gvs[PULL_EXISTS] >>
     qpat_assum `RTC _ c' s` $ strip_assume_tac o SRULE[RTC_PATH] >>
     Cases_on `!x. MEM x l ⇒ lookup visited' x = NONE` >>
     gvs[]
@@ -976,7 +973,7 @@ Proof
     >- (
       drule_then drule $ cj 1 by_super_aux_IMP_reachable >>
       disch_then $ qspec_then `EL n l` mp_tac >>
-      rw[GSYM mlmapTheory.lookup_thm] >>
+      rw[] >>
       Cases_on `n` >>
       gvs[] >>
       first_x_assum $ qspec_then `n'` mp_tac >>
@@ -997,24 +994,16 @@ Proof
   metis_tac[]
 QED
 
-(* every class in the super list must be a valid key of the map *)
-Definition super_keys_ok_def:
-  super_keys_ok cl_map =
-  (∀c clinfo c'.
-    mlmap$lookup cl_map c = SOME clinfo ∧ MEM c' clinfo.super ⇒
-    ∃x. mlmap$lookup cl_map c' = SOME x)
-End
-
 (* everything in the super list must be in the map *)
 Theorem well_formed_by_super_aux:
-  (∀cl_map visited c (t:'a) clinfo.
+  (∀(cl_map:'b class_map_impl) visited c (t:'a) clinfo.
     map_ok cl_map ∧ map_ok visited ∧
     super_keys_ok cl_map ⇒
     ((∃clinfo. mlmap$lookup cl_map c = SOME clinfo ∨
       (∃m. lookup visited c = SOME m)) ⇔
     (∃m. by_super_aux cl_map visited c t = SOME m))) ∧
 
-  ∀cl_map visited cs (t:'a).
+  ∀(cl_map:'b class_map_impl) visited cs (t:'a).
     map_ok cl_map ∧ map_ok visited ∧
     super_keys_ok cl_map ⇒
     ((∀c. MEM c cs ⇒
@@ -1074,15 +1063,19 @@ Definition by_super_def:
     by_super_aux cl_map (empty mlstring$compare) c t
 End
 
+Theorem lookup_empty:
+  map_ok (empty cmp: ('a,'b) mlmap$map) ⇒
+  lookup (empty cmp: ('a,'b) mlmap$map) k = NONE
+Proof
+  simp[mlmapTheory.lookup_thm,mlmapTheory.empty_thm]
+QED
+
 Theorem by_super_thm:
   by_super cl_map (c,t) = SOME visited ⇒
   (∀s v. (mlmap$lookup visited s = SOME v) ⇔
-    (v = t ∧
-      (c = s ∨ super_reachable (to_class_map cl_map) c s)))
+    (v = t ∧ super_reachable_RTC cl_map c s))
 Proof
-  simp[super_reachable_def,to_class_map_def,by_super_def,
-    FMAP_MAP2_THM,FLOOKUP_FMAP_MAP2,PULL_EXISTS,
-    GSYM RTC_CASES_TC] >>
+  simp[super_reachable_RTC_def,by_super_def] >>
   strip_tac >>
   `map_ok (empty mlstring$compare)` by
     simp[mlmapTheory.empty_thm,mlstringTheory.TotOrd_compare] >>
@@ -1093,14 +1086,14 @@ Proof
     >- (
       (drule_then $ drule_then irule) $
         cj 1 by_super_aux_lookup_preserve_type >>
-      simp[mlmapTheory.lookup_thm,mlmapTheory.empty_thm] >>
+      simp[lookup_empty] >>
       metis_tac[]
     ) >>
     drule_all $ cj 1 by_super_aux_IMP_reachable >>
-    simp[mlmapTheory.lookup_thm,mlmapTheory.empty_thm]
+    simp[lookup_empty]
   ) >>
   drule_then drule $ cj 1 super_reachable_IMP_by_super_aux >>
-  simp[mlmapTheory.lookup_thm,mlmapTheory.empty_thm] >>
+  simp[lookup_empty] >>
   rw[] >>
   first_x_assum drule >>
   metis_tac[]
@@ -1124,9 +1117,8 @@ Definition lookup_inst_map_def:
   lookup_inst_map inst_map c t =
   do
     (tcons,targs) <- split_ty_cons t;
-    inst_info <- lookup inst_map (c,tcons);
-    assert (LENGTH targs = inst_info.nargs);
-    return (inst_info.impl, MAP (I ## flip EL targs) inst_info.cstr)
+    inst_info <- lookup inst_map (c,tcons,LENGTH targs);
+    return (inst_info.impls, MAP (I ## flip EL targs) inst_info.cstr)
   od
 End
 
@@ -1134,76 +1126,97 @@ Definition by_inst_def:
   by_inst inst_map c t = OPTION_MAP SND $ lookup_inst_map inst_map c t
 End
 
-Theorem lookup_inst_map_lem:
-  ∀inst_map c t impl cstr.
-    lookup_inst_map inst_map c t = SOME (impl,cstr)
-    ⇔
-    (∃tcons targs inst_info.
-      split_ty_cons t = SOME (tcons,targs) ∧
-      lookup inst_map (c,tcons) = SOME inst_info ∧
-      LENGTH targs = inst_info.nargs ∧
-      impl = inst_info.impl ∧
-      cstr = MAP (I ## (λv. EL v targs)) inst_info.cstr)
+Theorem lookup_inst_map_tcons_to_type:
+  lookup_inst_map inst_map c t = SOME (impl,cstr) ⇔
+  (∃tcons targs inst_info.
+    t = tcons_to_type tcons targs ∧
+    lookup inst_map (c,tcons,LENGTH targs) =
+      SOME inst_info ∧
+    impl = inst_info.impls ∧
+    cstr = MAP (I ## (λv. EL v $ ty_args t)) inst_info.cstr)
 Proof
-  reverse $ rw[lookup_inst_map_def,EQ_IMP_THM]
-  >- simp[combinTheory.C_DEF] >>
-  pairarg_tac >>
+  rw[lookup_inst_map_def,EQ_IMP_THM,EXISTS_PROD]
+  >- (
+    drule_then (assume_tac o GSYM) tcons_to_type_split_ty_cons >>
+    first_assum $ irule_at (Pos hd) >>
+    simp[MAP_EQ_f,ty_args_cons_types,tcons_to_type_def,
+      FORALL_PROD,ty_args_alt]
+  ) >>
+  irule_at (Pos hd) split_ty_cons_tcons_to_type >>
+  simp[MAP_EQ_f,ty_args_cons_types,tcons_to_type_def,
+    FORALL_PROD,ty_args_alt]
+QED
+
+Theorem lookup_inst_map_thm:
+  lookup_inst_map inst_map c t = SOME (impl,cstr) ⇔
+  (∃tcons inst_info.
+    head_ty_cons t = SOME tcons ∧
+    lookup inst_map (c,tcons,LENGTH $ ty_args t) =
+      SOME inst_info ∧
+    impl = inst_info.impls ∧
+    cstr = MAP (I ## (λv. EL v $ ty_args t)) inst_info.cstr)
+Proof
+  rw[lookup_inst_map_def,EQ_IMP_THM,
+    split_ty_cons_thm,EXISTS_PROD] >>
   gvs[combinTheory.C_DEF]
 QED
 
 Theorem by_inst_lem:
   ∀inst_map c t cstr.
   by_inst inst_map c t = SOME cstr ⇔
-  (∃tcons targs inst_info.
-    split_ty_cons t = SOME (tcons,targs) ∧
-    lookup inst_map (c,tcons) = SOME inst_info ∧
-    LENGTH targs = inst_info.nargs ∧
-      cstr = MAP (I ## (λv. EL v targs)) inst_info.cstr)
+  (∃tcons inst_info.
+    head_ty_cons t = SOME tcons ∧
+    lookup inst_map (c,tcons,LENGTH $ ty_args t) =
+      SOME inst_info ∧
+    cstr = MAP (I ## (λv. EL v $ ty_args t)) inst_info.cstr)
 Proof
-  simp[by_inst_def,LAMBDA_PROD,GSYM PEXISTS_THM,lookup_inst_map_lem]
+  rw[by_inst_def,EQ_IMP_THM,EXISTS_PROD] >>
+  gvs[lookup_inst_map_thm]
 QED
 
-Theorem lookup_inst_map_thm:
-  ∀inst_map c t impl cstr.
-    lookup_inst_map inst_map c t = SOME (impl,cstr)
-    ⇔
-    (∃tcons targs inst_info.
-      split_ty_cons t = SOME (tcons,targs) ∧
-      lookup inst_map (c,tcons) = SOME inst_info ∧
-      LENGTH targs = inst_info.nargs ∧
-      impl = inst_info.impl ∧
-      LENGTH cstr = LENGTH inst_info.cstr ∧
-      (∀n. n < LENGTH inst_info.cstr ⇒
-        let (cl,v) = EL n inst_info.cstr in
-          EL n cstr = (cl,EL v targs)))
+(* Every type variable in the context is in the rhs *) 
+Definition well_scoped_inst_map_def:
+  well_scoped_inst_map (inst_map:'a inst_map_impl) =
+  (∀class tycons n inst_info c v.
+    lookup inst_map (class,tycons,n) = SOME inst_info ∧
+    MEM (c,v) inst_info.cstr ⇒
+    v < n)
+End
+
+Theorem inst_map_abs_rel_IMP_well_scoped_inst_map:
+  inst_map_abs_rel inst_map_impl inst_map_abs ∧
+  instance_list_kind_ok tds clk inst_map_abs ⇒
+  well_scoped_inst_map inst_map_impl
 Proof
-  reverse $ rw[lookup_inst_map_lem,EQ_IMP_THM]
-  >- (
-    simp[] >>
-    irule LIST_EQ >>
-    rw[EL_MAP,oneline PAIR_MAP_THM] >>
-    CASE_TAC >>
-    first_x_assum drule >>
-    simp[]
-  ) >>
+  rw[inst_map_abs_rel_def,well_scoped_inst_map_def] >>
+  last_x_assum drule >>
+  rw[inst_abs_rel_def] >>
+  drule $ SRULE[EVERY_MEM] $ iffLR instance_list_kind_ok_def >>
+  disch_then drule >>
+  rw[instance_kind_ok_def,entailment_kind_ok_def,
+    instance_to_entailment_def] >>
+  drule $ iffLR EVERY_MEM >>  
+  simp[MEM_MAP,PULL_EXISTS] >>
+  disch_then drule >>
   rw[] >>
-  pairarg_tac >>
-  gvs[EL_MAP,oneline PAIR_MAP_THM]
+  drule kind_ok_IMP_freetyvars_ok >>
+  simp[freetyvars_ok_def]
 QED
 
-Theorem by_inst_thm:
-  ∀inst_map c t cstr.
-    by_inst inst_map c t = SOME cstr ⇔
-    (∃tcons targs inst_info.
-      split_ty_cons t = SOME (tcons,targs) ∧
-      lookup inst_map (c,tcons) = SOME inst_info ∧
-      LENGTH targs = inst_info.nargs ∧
-      LENGTH cstr = LENGTH inst_info.cstr ∧
-      (∀n. n < LENGTH inst_info.cstr ⇒
-        let (cl,v) = EL n inst_info.cstr in
-          EL n cstr = (cl,EL v targs)))
+Theorem by_inst_subst:
+  well_scoped_inst_map inst_map ∧
+  by_inst inst_map c t = SOME ps ⇒
+  by_inst inst_map c (subst_db skip ts t) =
+    SOME (MAP (λ(c,t). (c,subst_db skip ts t)) ps)
 Proof
-  simp[by_inst_def,LAMBDA_PROD,GSYM PEXISTS_THM,lookup_inst_map_thm]
+  simp[by_inst_def,lookup_inst_map_def,EXISTS_PROD] >>
+  rw[split_ty_cons_thm,head_ty_cons_eq_head_ty] >>
+  simp[subst_db_head_ty,subst_db_ty_args,MAP_MAP_o,
+    combinTheory.o_DEF,lambdify PAIR_MAP,LAMBDA_PROD] >>
+  rw[MAP_EQ_f] >>
+  pairarg_tac >> gvs[] >>
+  drule_all $ iffLR well_scoped_inst_map_def >>
+  simp[EL_MAP]
 QED
 
 Inductive full_entail:
@@ -1211,7 +1224,8 @@ Inductive full_entail:
   MEM p ps ⇒ full_entail cl_map inst_map ps p
 [~super]
   full_entail cl_map inst_map ps (c,t) ∧
-  super_reachable cl_map c s ⇒
+  lookup cl_map c = SOME cl ∧
+  MEM s cl.supers ⇒
   full_entail cl_map inst_map ps (s,t)
 [~inst]
   by_inst inst_map c t = SOME qs ∧
@@ -1220,11 +1234,9 @@ Inductive full_entail:
 End
 
 Inductive entail:
-[~mem]
-  MEM p ps ⇒ entail cl_map inst_map ps p
 [~super]
   MEM (c,t) ps ∧
-  super_reachable cl_map c s ⇒
+  super_reachable_RTC cl_map c s ⇒
   entail cl_map inst_map ps (s,t)
 [~inst]
   by_inst inst_map c t = SOME qs ∧
@@ -1232,13 +1244,27 @@ Inductive entail:
   entail cl_map inst_map ps (c,t)
 End
 
-Definition well_scoped_inst_map_def:
-  well_scoped_inst_map inst_map =
-  (∀k inst_info c v.
-    lookup inst_map k = SOME inst_info ∧
-    MEM (c,v) inst_info.cstr ⇒
-    v < inst_info.nargs)
-End
+Theorem entail_strong_ind:
+  ∀cl_map inst_map ps entail'.
+    (∀c s t.
+      MEM (c,t) ps ∧ super_reachable_RTC cl_map c s ⇒ entail' (s,t)) ∧
+    (∀c qs t.
+      by_inst inst_map c t = SOME qs ∧ (∀q. MEM q qs ⇒
+        entail cl_map inst_map ps q ∧ entail' q) ⇒
+      entail' (c,t)) ⇒
+  ∀a0. entail cl_map inst_map ps a0 ⇒ entail' a0
+Proof
+  rpt gen_tac >>
+  strip_tac >>
+  `∀a0. entail cl_map inst_map ps a0 ⇒
+    entail' a0 ∧ entail cl_map inst_map ps a0` suffices_by rw[] >>
+  ho_match_mp_tac entail_ind >>
+  rw[]
+  >- metis_tac[]
+  >- drule_all_then irule entail_super >>
+  irule entail_inst >>
+  rw[]
+QED
 
 Theorem entail_tsubst:
   well_scoped_inst_map inst_map ⇒
@@ -1249,12 +1275,6 @@ Proof
   strip_tac >>
   ho_match_mp_tac entail_ind >>
   rw[]
-  >- (
-    irule entail_mem >>
-    simp[MEM_MAP] >>
-    first_x_assum $ irule_at (Pos last) >>
-    simp[]
-  )
   >- (
     irule entail_super >>
     simp[MEM_MAP,PULL_EXISTS] >>
@@ -1270,16 +1290,7 @@ Proof
     pairarg_tac >>
     gvs[]
   ) >>
-  gvs[by_inst_thm] >>
-  drule_then (irule_at (Pos hd)) split_ty_cons_tsubst >>
-  rw[] >>
-  first_x_assum drule >>
-  pairarg_tac >> gvs[EL_MAP] >>
-  DEP_REWRITE_TAC[EL_MAP] >>
-  gvs[well_scoped_inst_map_def] >>
-  last_x_assum irule >>
-  simp[MEM_EL] >>
-  metis_tac[]
+  gvs[by_inst_subst]
 QED
 
 Theorem full_entail_tsubst:
@@ -1299,7 +1310,6 @@ Proof
   )
   >- (
     irule full_entail_super >>
-    simp[MEM_MAP,PULL_EXISTS] >>
     first_assum $ irule_at (Pos last) >>
     first_assum $ irule_at (Pos last) >>
     simp[]
@@ -1312,16 +1322,7 @@ Proof
     pairarg_tac >>
     gvs[]
   ) >>
-  gvs[by_inst_thm] >>
-  drule_then (irule_at (Pos hd)) split_ty_cons_tsubst >>
-  rw[] >>
-  first_x_assum drule >>
-  pairarg_tac >> gvs[EL_MAP] >>
-  DEP_REWRITE_TAC[EL_MAP] >>
-  gvs[well_scoped_inst_map_def] >>
-  last_x_assum irule >>
-  simp[MEM_EL] >>
-  metis_tac[]
+  gvs[by_inst_subst]
 QED
 
 (* `entail` is equivalent to `full_entail`
@@ -1330,27 +1331,34 @@ QED
 * `entail`s (s,t) for all super class s of c *)
 Definition entail_wf_def:
   entail_wf cl_map inst_map ⇔
-  ∀c tcons inst clinfo s.
-    lookup inst_map (c,tcons) = SOME inst ∧
-    FLOOKUP cl_map c = SOME clinfo ∧ MEM s clinfo.super ⇒
-    ∃inst'. lookup inst_map (s,tcons) = SOME inst' ∧
-    inst'.nargs = inst.nargs ∧
-    ∀cl v. MEM (cl,v) inst'.cstr ⇒
-      MEM (cl,v) inst.cstr ∨
-      ∃scl. MEM (scl,v) inst.cstr ∧ super_reachable cl_map scl cl
+  ∀c tcons n inst clinfo s.
+    lookup inst_map (c,tcons,n) = SOME inst ∧
+    lookup cl_map c = SOME clinfo ∧ MEM s clinfo.supers ⇒
+    ∃inst'. lookup inst_map (s,tcons,n) = SOME inst' ∧
+      (∀cl v. MEM (cl,v) inst'.cstr ⇒
+        ∃scl. MEM (scl,v) inst.cstr ∧
+          super_reachable_RTC cl_map scl cl)
 End
 
+(* every class in the constraints is in cl_map *)
+Definition inst_map_constraints_class_ok_def:
+  inst_map_constraints_class_ok cl_map inst_map ⇔
+  (∀k inst cl tyvar.
+    lookup inst_map k = SOME inst ∧ MEM (cl,tyvar) inst.cstr ⇒
+      ∃clinfo. lookup cl_map cl = SOME clinfo)
+End
+
+(* implementation to check if entail_wf is satified *)
 Definition entail_wf_impl_def:
   entail_wf_impl cl_map inst_map ⇔
-  all (λk inst.
-    case lookup cl_map (FST k) of
+  all (λ(class,tycons,ntargs) inst.
+    case lookup cl_map class of
     | NONE => T
     | SOME clinfo =>
         EVERY (λs.
-          case lookup inst_map (s,SND k) of
+          case lookup inst_map (s,tycons,ntargs) of
           | NONE => F
           | SOME inst' =>
-              inst'.nargs = inst.nargs ∧
               let supers = MAP (by_super cl_map) inst.cstr in
               EVERY (λclv.
                 EXISTS (λx.
@@ -1358,31 +1366,20 @@ Definition entail_wf_impl_def:
                   | NONE => F
                   | SOME visited =>
                       lookup visited (FST clv) = SOME (SND clv))
-                supers) inst'.cstr) clinfo.super) inst_map
-End
-
-Definition inst_map_constraints_ok_def:
-  inst_map_constraints_ok cl_map inst_map ⇔
-  (∀k inst x.
-    lookup inst_map k = SOME inst ∧ MEM x inst.cstr ⇒
-      ∃clinfo. lookup cl_map (FST x) = SOME clinfo)
+                supers) inst'.cstr) clinfo.supers) inst_map
 End
 
 Theorem entail_wf_impl_thm:
   map_ok cl_map ∧ map_ok inst_map ∧
-  super_keys_ok cl_map ∧ inst_map_constraints_ok cl_map inst_map ⇒
+  super_keys_ok cl_map ∧ inst_map_constraints_class_ok cl_map inst_map ⇒
   (entail_wf_impl cl_map inst_map ⇔
-    entail_wf (to_class_map cl_map) inst_map)
+    entail_wf cl_map inst_map)
 Proof
   rw[entail_wf_impl_def,all_thm,entail_wf_def,EQ_IMP_THM]
   >- (
     first_x_assum drule >>
     simp[] >>
-    TOP_CASE_TAC
-    >- gvs[to_class_map_def,FLOOKUP_FMAP_MAP2,FMAP_MAP2_THM,
-      mlmapTheory.lookup_thm] >>
     rw[EVERY_MEM] >>
-    gvs[FLOOKUP_to_class_map] >>
     first_x_assum drule >>
     TOP_CASE_TAC >>
     rw[] >>
@@ -1394,12 +1391,10 @@ Proof
     rename1`by_super cl_map ct = SOME _` >>
     Cases_on `ct` >>
     drule_all $ iffLR by_super_thm >>
-    rw[] >>
     metis_tac[]
   ) >>
-  rename1 `lookup inst_map k = SOME _` >>
-  Cases_on `k` >>
-  gvs[FLOOKUP_to_class_map,EVERY_MEM,PULL_EXISTS] >>
+  pairarg_tac >>
+  gvs[EVERY_MEM,PULL_EXISTS] >>
   TOP_CASE_TAC >>
   rpt strip_tac >>
   first_x_assum drule_all >>
@@ -1408,35 +1403,18 @@ Proof
   rename1 `MEM clv inst'.cstr` >>
   Cases_on `clv` >>
   first_x_assum drule >>
-  rw[]
-  >- (
-    first_assum $ irule_at (Pos hd) >>
-    rename1 `by_super cl_map (c',t')` >>
-    TOP_CASE_TAC
-    >- (
-      drule_all $ iffLR inst_map_constraints_ok_def >>
-      rpt strip_tac >>
-      fs[] >>
-      drule_all_then (qspec_then `t'` strip_assume_tac) $
-        SRULE[PULL_EXISTS] $ iffLR well_formed_by_super >>
-      gvs[]) >>
-    drule_then irule $ iffRL by_super_thm >>
-    rw[]
-  ) >>
-  first_x_assum $ irule_at (Pos hd) >>
-  rename1 `by_super cl_map (c',t')` >>
+  rw[] >>
+  first_assum $ irule_at (Pos hd) >>
+  rename1 `by_super cl_map (scl,t')` >>
   TOP_CASE_TAC
   >- (
-    `∃x. lookup cl_map c' = SOME x`
-    by (
-      gvs[super_reachable_def] >>
-      drule TC_CASES1_E >>
-      rw[FLOOKUP_to_class_map] >>
-      metis_tac[]
-    ) >>
-    drule_all_then (qspec_then `t'` strip_assume_tac) $
-      SRULE[PULL_EXISTS] $ iffLR well_formed_by_super >>
-    gvs[]
+    `∃x. by_super cl_map (scl,t') = SOME x`
+      suffices_by gvs[] >>
+    irule $ iffLR well_formed_by_super >>
+    simp[] >>
+    drule_then irule $
+      iffLR inst_map_constraints_class_ok_def >>
+    metis_tac[]
   ) >>
   drule_then irule $ iffRL by_super_thm >>
   rw[]
@@ -1444,43 +1422,42 @@ QED
 
 Theorem entail_super_TypeVar:
   well_scoped_inst_map inst_map ∧
-  lookup inst_map (c,tcons) = SOME inst ∧
-  FLOOKUP cl_map c = SOME clinfo ∧
-  MEM s clinfo.super ⇒
+  lookup inst_map (c,tcons,ntargs) = SOME inst ∧
+  lookup cl_map c = SOME clinfo ∧
+  MEM s clinfo.supers ⇒
   (entail cl_map inst_map (MAP (I ## TypeVar) inst.cstr)
-    (s,tcons_to_type tcons (GENLIST TypeVar inst.nargs)) ⇔
-   ∃inst'. lookup inst_map (s,tcons) = SOME inst' ∧
-    inst'.nargs = inst.nargs ∧
+    (s,tcons_to_type tcons (GENLIST TypeVar ntargs)) ⇔
+   ∃inst'.
+    lookup inst_map (s,tcons,ntargs) = SOME inst' ∧
     ∀cl v. MEM (cl,v) inst'.cstr ⇒
-      MEM (cl,v) inst.cstr ∨
-      ∃scl. MEM (scl,v) inst.cstr ∧ super_reachable cl_map scl cl)
+      ∃scl. MEM (scl,v) inst.cstr ∧
+        super_reachable_RTC cl_map scl cl)
 Proof
   rw[EQ_IMP_THM]
   >- (
     reverse $ pop_assum $ strip_assume_tac o SRULE[Once entail_cases]
     >- (
-      gvs[by_inst_lem,split_ty_cons_tcons_to_type,MEM_MAP,PULL_EXISTS] >>
+      gvs[by_inst_def,lookup_inst_map_def,
+        split_ty_cons_tcons_to_type,MEM_MAP,PULL_EXISTS] >>
       rw[] >>
-      `v < inst_info.nargs` by (
+      `v < ntargs` by (
         gvs[well_scoped_inst_map_def] >>
         last_x_assum irule >>
-        metis_tac[MEM_EL]) >>
+        metis_tac[MEM_EL]
+      ) >>
       first_x_assum drule >>
       rw[Once entail_cases] >>
       gvs[MEM_MAP]
       >- (
         rename1 `MEM p inst.cstr` >>
         Cases_on `p` >>
-        gvs[]
-      )
-      >- (
-        rename1 `MEM p inst.cstr` >>
-        Cases_on `p` >>
         gvs[] >>
-        disj2_tac >>
-        metis_tac[]
+        metis_tac[super_reachable_RTC_CASES_super_reachable]
       ) >>
-      gvs[by_inst_lem,split_ty_cons_thm,head_ty_cons_def]
+      gvs[by_inst_def,lookup_inst_map_def] >>
+      rename1 `split_ty_cons _ = SOME p` >>
+      Cases_on `p` >>
+      gvs[split_ty_cons_thm,head_ty_cons_def]
     ) >>
     gvs[MEM_MAP] >>
     rename1 `MEM p inst.cstr` >>
@@ -1488,20 +1465,10 @@ Proof
     gvs[tcons_to_type_NEQ_TypeVar]
   ) >>
   irule entail_inst >>
-  rw[by_inst_lem,split_ty_cons_tcons_to_type,MEM_MAP,PULL_EXISTS] >>
-  rename1 `entail _ _ _ (_ p)` >>
-  Cases_on `p` >>
+  rw[by_inst_def,lookup_inst_map_def,EXISTS_PROD,
+    split_ty_cons_tcons_to_type,MEM_MAP,PULL_EXISTS] >>
   first_x_assum drule >>
-  rw[]
-  >- (
-    irule entail_mem >>
-    simp[MEM_MAP] >>
-    first_assum $ irule_at (Pos last) >>
-    DEP_REWRITE_TAC[EL_GENLIST] >>
-    gvs[well_scoped_inst_map_def] >>
-    last_x_assum irule >>
-    metis_tac[MEM_EL]
-  ) >>
+  rw[] >>
   irule entail_super >>
   simp[MEM_MAP] >>
   first_assum $ irule_at (Pos last) >>
@@ -1516,11 +1483,11 @@ QED
 Theorem entail_wf_alt:
   well_scoped_inst_map inst_map ⇒
   (entail_wf cl_map inst_map ⇔
-  ∀c tcons inst clinfo s.
-    lookup inst_map (c,tcons) = SOME inst ∧
-    FLOOKUP cl_map c = SOME clinfo ∧ MEM s clinfo.super ⇒
+  ∀c tcons ntargs inst clinfo s.
+    lookup inst_map (c,tcons,ntargs) = SOME inst ∧
+    lookup cl_map c = SOME clinfo ∧ MEM s clinfo.supers ⇒
     entail cl_map inst_map (MAP (I ## TypeVar) inst.cstr)
-      (s,tcons_to_type tcons (GENLIST TypeVar inst.nargs)))
+      (s,tcons_to_type tcons (GENLIST TypeVar ntargs)))
 Proof
   rw[entail_wf_def,EQ_IMP_THM]
   >- (
@@ -1534,14 +1501,13 @@ QED
 
 Triviality entail_wf_lookup_super:
   entail_wf cl_map inst_map ∧
-  FLOOKUP cl_map c = SOME c' ∧
-  MEM s c'.super ∧
-  lookup inst_map (c,tcons) = SOME inst ⇒
-  ∃inst'. lookup inst_map (s,tcons) = SOME inst' ∧
-    inst'.nargs = inst.nargs ∧
+  lookup cl_map c = SOME c' ∧
+  MEM s c'.supers ∧
+  lookup inst_map (c,tcons,ntargs) = SOME inst ⇒
+  ∃inst'. lookup inst_map (s,tcons,ntargs) = SOME inst' ∧
     ∀cl v. MEM (cl,v) inst'.cstr ⇒
-      MEM (cl,v) inst.cstr ∨
-      ∃scl. MEM (scl,v) inst.cstr ∧ super_reachable cl_map scl cl
+      ∃scl. MEM (scl,v) inst.cstr ∧
+        super_reachable_RTC cl_map scl cl
 Proof
   rw[] >>
   gvs[entail_wf_def] >>
@@ -1549,102 +1515,113 @@ Proof
   gvs[]
 QED
 
+Theorem super_reachable_RTC_trans:
+  super_reachable_RTC cl_map x y ∧
+  super_reachable_RTC cl_map y z ⇒
+  super_reachable_RTC cl_map x z
+Proof
+  rw[super_reachable_RTC_CASES_super_reachable] >>
+  simp[] >>
+  gvs[super_reachable_def] >>
+  drule_all $ cj 2 TC_RULES >>
+  simp[]
+QED
+
 Theorem entail_wf_lookup_super_reachable:
   entail_wf cl_map inst_map ⇒
-  ∀c s. super_reachable cl_map c s ⇒
-  ∀tcons inst. lookup inst_map (c,tcons) = SOME inst ⇒
-  ∃inst'. lookup inst_map (s,tcons) = SOME inst' ∧
-    inst'.nargs = inst.nargs ∧
+  ∀c s. super_reachable_RTC cl_map c s ⇒
+  ∀tcons ntargs inst.
+    lookup inst_map (c,tcons,ntargs) = SOME inst ⇒
+  ∃inst'. lookup inst_map (s,tcons,ntargs) = SOME inst' ∧
     ∀cl v. MEM (cl,v) inst'.cstr ⇒
-      MEM (cl,v) inst.cstr ∨
-      ∃scl. MEM (scl,v) inst.cstr ∧ super_reachable cl_map scl cl
+      ∃scl. MEM (scl,v) inst.cstr ∧
+        super_reachable_RTC cl_map scl cl
 Proof
   strip_tac >>
-  simp[Once super_reachable_def] >>
-  ho_match_mp_tac TC_INDUCT_LEFT1 >>
+  simp[super_reachable_RTC_def] >>
+  ho_match_mp_tac RTC_INDUCT >>
   rw[]
-  >- metis_tac[entail_wf_lookup_super] >>
+  >- metis_tac[RTC_REFL] >>
   drule_all entail_wf_lookup_super >>
   rw[] >>
   last_x_assum drule >> rw[] >>
   rw[] >>
   first_x_assum drule >> rw[] >>
-  first_x_assum drule >> rw[]
-  >- metis_tac[] >>
-  disj2_tac >>
-  irule_at (Pos last) super_reachable_trans >>
-  metis_tac[]
+  first_x_assum drule >> rw[] >>
+  gvs[GSYM super_reachable_RTC_def] >>
+  metis_tac[super_reachable_RTC_trans]
 QED
 
-Theorem entail_strong_ind:
-  ∀cl_map inst_map ps entail'.
-    (∀p. MEM p ps ⇒ entail' p) ∧
-    (∀c s t.
-      MEM (c,t) ps ∧ super_reachable cl_map c s ⇒ entail' (s,t)) ∧
-    (∀c qs t.
-      by_inst inst_map c t = SOME qs ∧ (∀q. MEM q qs ⇒
-        entail cl_map inst_map ps q ∧ entail' q) ⇒
-      entail' (c,t)) ⇒
-  ∀a0. entail cl_map inst_map ps a0 ⇒ entail' a0
-Proof
-  rpt gen_tac >>
-  strip_tac >>
-  `∀a0. entail cl_map inst_map ps a0 ⇒
-    entail' a0 ∧ entail cl_map inst_map ps a0` suffices_by rw[] >>
-  ho_match_mp_tac entail_ind >>
-  rw[]
-  >- drule_all_then irule entail_mem
-  >- metis_tac[]
-  >- drule_all_then irule entail_super >>
-  irule entail_inst >>
-  rw[]
-QED
-
-Triviality entail_wf_super_reachable':
+Triviality entail_wf_super_reachable_RTC_aux:
   entail_wf cl_map inst_map ⇒
   ∀p. entail cl_map inst_map ps p ⇒
     ∀c t clinfo s. p = (c,t) ∧
-    (c = s ∨
-    super_reachable cl_map c s) ⇒
+    super_reachable_RTC cl_map c s ⇒
     entail cl_map inst_map ps (s,t)
 Proof
   strip_tac >>
   ho_match_mp_tac entail_strong_ind >>
   rw[]
-  >- drule_then irule entail_mem
-  >- drule_all_then irule entail_super
-  >- drule_all_then irule entail_super
   >- (
     irule entail_super >>
     first_assum $ irule_at (Pos hd) >>
-    drule_all_then irule super_reachable_trans) >>
+    drule_all_then irule super_reachable_RTC_trans
+  ) >>
   gvs[IMP_CONJ_THM,FORALL_AND_THM] >>
-  gvs[PULL_FORALL,AND_IMP_INTRO]
-  >- drule_all_then irule entail_inst >>
+  gvs[PULL_FORALL,AND_IMP_INTRO] >>
+  (* drule_all entail_inst >> *)
   gvs[by_inst_lem,MEM_MAP,PULL_EXISTS,LAMBDA_PROD,
     GSYM PFORALL_THM,GSYM PEXISTS_THM] >>
   irule entail_inst >>
   simp[by_inst_lem,MEM_MAP,
-    PULL_EXISTS,LAMBDA_PROD,GSYM PFORALL_THM] >>
+    PULL_EXISTS,EXISTS_PROD,GSYM PFORALL_THM] >>
   drule_all entail_wf_lookup_super_reachable >>
   rw[] >>
-  rw[MEM_MAP,GSYM PEXISTS_THM] >>
-  first_x_assum drule >>
-  rw[] >>
-  first_x_assum drule >> rw[]
+  rw[MEM_MAP,GSYM PEXISTS_THM]
+QED
+
+Theorem entail_wf_super_reachable_RTC:
+  entail_wf cl_map inst_map ∧
+  entail cl_map inst_map ps (c,t) ∧
+  super_reachable_RTC cl_map c s ⇒
+  entail cl_map inst_map ps (s,t)
+Proof
+  metis_tac[entail_wf_super_reachable_RTC_aux]
 QED
 
 Theorem entail_wf_super_reachable:
-  ∀cl_map inst_map ps c t s.
-    entail_wf cl_map inst_map ∧
-    entail cl_map inst_map ps (c,t) ∧
-    super_reachable cl_map c s ⇒
-    entail cl_map inst_map ps (s,t)
+  entail_wf cl_map inst_map ∧
+  entail cl_map inst_map ps (c,t) ∧
+  super_reachable cl_map c s ⇒
+  entail cl_map inst_map ps (s,t)
 Proof
-  metis_tac[entail_wf_super_reachable']
+  rw[] >>
+  (drule_then $ drule_then irule)
+    entail_wf_super_reachable_RTC >>
+  simp[super_reachable_RTC_CASES_super_reachable]
 QED
 
-Theorem entail_eq_full_entail:
+Theorem super_reachable_IMP_full_entail:
+  ∀c s. super_reachable cl_map c s ⇒
+  MEM (c,t) ps ⇒
+  full_entail cl_map inst_map ps (s,t)
+Proof
+  simp[super_reachable_def] >>
+  ho_match_mp_tac TC_INDUCT_RIGHT1 >>
+  rw[]
+  >- (
+    irule full_entail_super >>
+    first_assum $ irule_at (Pos hd) >>
+    simp[] >>
+    drule_then irule full_entail_mem
+  ) >>
+  gvs[] >>
+  irule full_entail_super >>
+  first_assum $ irule_at (Pos hd) >>
+  simp[]
+QED
+
+Theorem entail_EQ_full_entail:
   entail_wf cl_map inst_map ⇒
   ∀p. (entail cl_map inst_map ps p ⇔ full_entail cl_map inst_map ps p)
 Proof
@@ -1653,18 +1630,28 @@ Proof
   conj_tac
   >- (
     ho_match_mp_tac entail_ind >>
-    rw[]
+    rw[super_reachable_RTC_CASES_super_reachable]
     >- drule_all_then irule full_entail_mem
     >- (
-      drule_at_then (Pos last) irule full_entail_super >>
-      drule_then irule full_entail_mem
+      drule_all_then irule
+        super_reachable_IMP_full_entail
     )
     >- drule_all_then irule full_entail_inst
   ) >>
   ho_match_mp_tac full_entail_ind >>
   rw[]
-  >- drule_all_then irule entail_mem
-  >- drule_all_then irule entail_wf_super_reachable
+  >- (
+    Cases_on `p` >>
+    irule entail_super >>
+    metis_tac[super_reachable_RTC_def,RTC_REFL]
+  )
+  >- (
+    drule_then irule entail_wf_super_reachable >>
+    first_assum $ irule_at (Pat `entail _ _ _ _`) >>
+    simp[super_reachable_def] >>
+    irule $ cj 1 TC_RULES >>
+    simp[]
+  )
   >- drule_all_then irule entail_inst
 QED
 
@@ -1675,7 +1662,6 @@ Theorem entail_monotone:
 Proof
   ho_match_mp_tac entail_ind >>
   rw[]
-  >- (irule entail_mem >> metis_tac[])
   >- (irule entail_super >> metis_tac[]) >>
   irule entail_inst >> metis_tac[]
 QED
@@ -1711,7 +1697,7 @@ Definition entail_aux_def:
   (entail_aux supers inst_map (c,t) =
     if well_scoped_inst_map inst_map
     then
-      (EXISTS (\visited. lookup visited c = SOME t) supers ∨
+      (EXISTS (λvisited. lookup visited c = SOME t) supers ∨
       (case by_inst inst_map c t of
         | NONE => F
         | SOME qs => entail_aux_list supers inst_map qs))
@@ -1731,7 +1717,8 @@ Termination
      | INL _ => 0))` >>
   rw[]
   >- (
-    gvs[by_inst_lem] >>
+    gvs[by_inst_def,lookup_inst_map_def] >>
+    pairarg_tac >> gvs[] >>
     PURE_REWRITE_TAC[Once $ GSYM arithmeticTheory.GREATER_DEF] >>
     irule list_max_intro >>
     simp[EVERY_MAP,arithmeticTheory.GREATER_DEF,type_size_GT_0] >>
@@ -1814,7 +1801,7 @@ Theorem entail_aux_thm:
   (∀n. n < LENGTH ps ⇒
     by_super cl_map (EL n ps) = SOME (EL n supers)) ⇒
   (entail_aux supers inst_map p ⇔
-    entail (to_class_map cl_map) inst_map ps p)
+    entail cl_map inst_map ps p)
 Proof
   ho_match_mp_tac entail_aux_induct_EVERY >>
   rw[] >>
@@ -1831,9 +1818,9 @@ Proof
     first_x_assum $ drule_then assume_tac >>
     Cases_on `EL n ps` >>
     drule_all $ iffLR by_super_thm >>
-    rw[]
-    >- (irule entail_mem >> metis_tac[MEM_EL]) >>
-    irule entail_super >> metis_tac[MEM_EL]
+    rw[] >>
+    irule entail_super >>
+    metis_tac[MEM_EL]
   )
   >- (
     pop_assum mp_tac >>
@@ -1854,20 +1841,24 @@ Proof
 QED
 
 Theorem entail_impl_thm:
-  map_ok cl_map ∧ map_ok inst_map ∧
+  map_ok cl_map ∧
+  map_ok inst_map ∧
   well_scoped_inst_map inst_map ∧ super_keys_ok cl_map ∧
   (∀q. MEM q ps ⇒ ∃clinfo. lookup cl_map (FST q) = SOME clinfo) ⇒
   entail_impl cl_map inst_map ps p =
-    entail (to_class_map cl_map) inst_map ps p
+    entail cl_map inst_map ps p
 Proof
   rw[oneline entail_impl_def] >>
   ntac 2 TOP_CASE_TAC
   >- (
     dxrule_then strip_assume_tac OPT_MMAP_NONE >>
     first_assum $ drule_then strip_assume_tac >>
-    drule_all_then (qspec_then `SND x` mp_tac) $
-      SRULE[PULL_EXISTS] $ iffLR well_formed_by_super >>
-    rw[]
+    spose_not_then kall_tac >>
+    `∃y. by_super cl_map x = SOME y`
+      suffices_by gvs[] >>
+    Cases_on `x` >>
+    irule $ SRULE[PULL_EXISTS] $ iffLR well_formed_by_super >>
+    gvs[]
   ) >>
   dxrule_then strip_assume_tac OPT_MMAP_SOME_EL >>
   irule entail_aux_thm >>
@@ -1877,22 +1868,244 @@ QED
 Theorem entail_impl_full_entail:
   map_ok cl_map ∧ map_ok inst_map ∧
   well_scoped_inst_map inst_map ∧ super_keys_ok cl_map ∧
-  entail_wf (to_class_map cl_map) inst_map ∧
+  entail_wf cl_map inst_map ∧
   (∀q. MEM q ps ⇒ ∃clinfo. lookup cl_map (FST q) = SOME clinfo) ⇒
   entail_impl cl_map inst_map ps p =
-    full_entail (to_class_map cl_map) inst_map ps p
+    full_entail cl_map inst_map ps p
 Proof
-  metis_tac[entail_impl_thm,entail_eq_full_entail]
+  metis_tac[entail_impl_thm,entail_EQ_full_entail]
 QED
 
-Theorem entail_IMP_has_dict:
+(* full_entail is an implmentation of has_dict, when the ie is
+* generated by the superclasses in cl_map_impl and
+* instances in inst_map_impl *)
+Theorem full_entail_IMP_has_dict:
+  class_map_kind_ok tds cl_map_abs ∧
+  instance_list_kind_ok tds clk inst_map_abs ∧
+  class_map_super_abs_rel cl_map_impl cl_map_abs ∧
+  inst_map_abs_rel inst_map_impl inst_map_abs ∧
+  EVERY (λ(c,t). ∃k. clk c = SOME k ∧ kind_ok tds ks k t) lie ∧
+  clk = class_map_to_clk cl_map_abs ∧
+  ie = set (MAP SND (class_map_to_ie cl_map_abs)) ∪
+    set (MAP SND (instance_list_to_ie inst_map_abs)) ∧
+  lie_set = set lie
+  ⇒
+  ∀p. full_entail cl_map_impl inst_map_impl lie p ⇒
+    ∀k. clk (FST p) = SOME k ∧ kind_ok tds ks k (SND p) ⇒
+  has_dict tds ks ie lie_set p
 Proof
+  strip_tac >>
+  ho_match_mp_tac full_entail_strongind >>
+  rw[super_reachable_RTC_CASES_super_reachable]
+  >- drule_then irule has_dict_lie
+  >- (
+    irule has_dict_ie >>
+    irule_at (Pat `_ ∈ _`) $ cj 1 $
+      PURE_REWRITE_RULE[SUBSET_DEF] SUBSET_UNION >>
+    gvs[MEM_MAP,PULL_EXISTS,class_map_to_ie_def,
+      LIST_BIND_def,MEM_FLAT] >>
+    dxrule_then (qspec_then `c` mp_tac) $
+      iffLR class_map_super_abs_rel_def >>
+    rw[OPTREL_def,class_super_abs_rel_def,EXTENSION] >>
+    drule_then assume_tac ALOOKUP_MEM >>
+    first_assum $ irule_at (Pat `MEM _ cl_map_abs`) >>
+    gvs[MEM_MAP,class_to_entailments_def,PULL_EXISTS,
+      EXISTS_PROD] >>
+    first_assum $ irule_at (Pat `MEM _ _.supers`) >>
+    simp[specialises_inst_def,PULL_EXISTS,subst_db_def,
+      EXISTS_PROD] >>
+    conj_tac
+    >- (
+      gvs[class_map_kind_ok_def] >>
+      last_x_assum drule >>
+      simp[super_classes_def,EVERY_MAP] >>
+      rw[EVERY_MEM] >>
+      first_x_assum drule >>
+      rw[] >> gvs[class_map_to_clk_def]
+    ) >>
+    irule has_dict_dicts >>
+    rw[] >>
+    first_x_assum irule >>
+    gvs[class_map_to_clk_def] >>
+    drule $ iffLR class_map_kind_ok_def >>
+    rw[] >>
+    pop_assum drule >>
+    simp[super_classes_def,EVERY_MAP] >>
+    rw[EVERY_MEM] >>
+    first_x_assum drule >>
+    rw[class_map_to_clk_def] >>
+    gvs[]
+  ) >>
+  irule has_dict_ie >>
+  irule_at (Pat `_ ∈ _`) $ cj 2 $
+    PURE_REWRITE_RULE[SUBSET_DEF] SUBSET_UNION >>
+  gvs[MEM_MAP,PULL_EXISTS,instance_list_to_ie_def] >>
+  gvs[by_inst_def] >>
+  rename1 `lookup_inst_map _ _ _ = SOME q` >>
+  PairCases_on `q` >>
+  gvs[lookup_inst_map_tcons_to_type,MEM_MAP,PULL_EXISTS] >>
+  drule_then drule $ cj 1 $ iffLR inst_map_abs_rel_def >>
+  rw[inst_abs_rel_def,instance_list_to_ie_def,MEM_MAP,
+    PULL_EXISTS] >>
+  first_assum $ irule_at (Pat `MEM _ inst_map_abs`) >>
+  qexists_tac `MAP (I ## flip EL targs) inst_info.cstr` >>
+  simp[instance_to_entailment_def,specialises_inst_def,
+    PULL_EXISTS,EVERY2_MAP,LAMBDA_PROD] >>
+  gvs[tcons_to_type_def,subst_db_cons_types,subst_db_def,
+    cons_types_Atom_EQ] >>
+  qexists `targs` >>
+  gvs[kind_ok_cons_types] >>
+  drule $ iffLR instance_list_kind_ok_def >>
+  disch_then $ drule o SRULE[EVERY_MEM] >>
+  simp[instance_kind_ok_def,instance_to_entailment_def,
+    entailment_kind_ok_def,EVERY_MAP,kind_ok_cons_types] >>
+  strip_tac >>
+  `kind_arrows ks' k = kind_arrows ks'' k`
+  by (
+    Cases_on `tcons` >>
+    gvs[kind_ok] >>
+    rename1 `Atom (TypeCons (INR builtin_ty))` >>
+    Cases_on `builtin_ty` >>
+    gvs[kind_ok] >>
+    rename1 `Atom (CompPrimTy comp)` >>
+    Cases_on `comp` >>
+    gvs[kind_ok]
+  ) >>
+  gvs[kind_arrows_ret_EQ] >>
+  `abs.kinds = ks'`
+  by (
+    gvs[LIST_REL_EL_EQN] >>
+    rw[LIST_EQ_REWRITE] >>
+    first_x_assum drule >>
+    simp[kind_ok,LLOOKUP_THM]
+  ) >>
+  rw[LIST_EQ_REWRITE,SF ETA_ss]
+  >- simp[EL_MAP,subst_db_def]
+  >- (
+    irule EVERY2_refl >>
+    simp[FORALL_PROD] >>
+    rpt strip_tac >>
+    rename1 `MEM (cstr_c,cstr_t) inst_info.cstr` >>
+    `cstr_t < LENGTH targs` suffices_by simp[] >>
+    drule $ iffLR instance_list_kind_ok_def >>
+    rw[EVERY_MEM] >>
+    first_x_assum drule >>
+    simp[instance_kind_ok_def,entailment_kind_ok_def,
+      instance_to_entailment_def] >>
+    rw[EVERY_MAP] >>
+    drule_then drule $ iffLR EVERY_MEM >>
+    rw[] >>
+    drule kind_ok_IMP_freetyvars_ok >>
+    simp[freetyvars_ok_def]
+  )
+  >- (
+    irule has_dict_dicts >>
+    rw[MEM_MAP] >>
+    last_x_assum drule >>
+    rw[MAP_MAP_o,combinTheory.o_DEF,ty_args_alt,
+      ty_args_cons_types,combinTheory.C_DEF] >>
+    simp[GSYM instance_to_entailment_def] >>
+    first_x_assum irule >>
+    drule_then drule $ iffLR EVERY_MEM >>
+    simp[LAMBDA_PROD] >>
+    pairarg_tac >> simp[] >>
+    pairarg_tac >> gvs[] >>
+    rw[kind_ok,LLOOKUP_THM] >>
+    gvs[LIST_REL_EL_EQN]
+  )
 QED
 
-Theorem has_dict_IMP_entail:
+Theorem has_dict_IMP_full_entail:
+  ALL_DISTINCT (MAP FST cl_map_abs) ∧
+  class_map_kind_ok tds cl_map_abs ∧
+  instance_list_kind_ok tds clk inst_map_abs ∧
+  class_map_super_abs_rel cl_map_impl cl_map_abs ∧
+  inst_map_abs_rel inst_map_impl inst_map_abs ∧
+  EVERY (λ(c,t). ∃k. clk c = SOME k ∧ kind_ok tds ks k t) lie ∧
+  clk = class_map_to_clk cl_map_abs ∧
+  ie = set (MAP SND (class_map_to_ie cl_map_abs)) ∪
+    set (MAP SND (instance_list_to_ie inst_map_abs)) ∧
+  lie_set = set lie
+  ⇒
+  (∀p. has_dict tds ks ie lie_set p ⇒
+    ∀k. clk (FST p) = SOME k ∧ kind_ok tds ks k (SND p) ⇒
+  full_entail cl_map_impl inst_map_impl lie p) ∧
+  (∀ps. has_dicts tds ks ie lie_set ps ⇒
+    ∀p k. MEM p ps ∧
+      clk (FST p) = SOME k ∧ kind_ok tds ks k (SND p) ⇒
+    full_entail cl_map_impl inst_map_impl lie p)
 Proof
+  strip_tac >>
+  ho_match_mp_tac has_dict_ind >>
+  rw[]
+  >- drule_then irule full_entail_mem
+  >- ( (* super class *)
+    gvs[MEM_MAP,PULL_EXISTS,class_map_to_ie_def,LIST_BIND_def,
+      MEM_FLAT] >>
+    drule $ iffLR class_map_kind_ok_def >>
+    simp[] >>
+    rename1 `MEM cl cl_map_abs` >>
+    PairCases_on `cl` >>
+    disch_then drule >>
+    drule $ iffLR class_map_super_abs_rel_def >>
+    drule_all_then strip_assume_tac ALOOKUP_ALL_DISTINCT_MEM >>
+    disch_then $ qspec_then `cl0` mp_tac >>
+    rw[OPTREL_def,super_classes_def,EVERY_MAP,EXTENSION,
+      class_super_abs_rel_def] >>
+    gvs[class_to_entailments_def,MEM_MAP,PULL_EXISTS,
+      EXISTS_PROD,specialises_inst_def] >>
+    qpat_x_assum `EVERY _ _.supers` $ drule o SRULE[EVERY_MEM] >>
+    strip_tac >>
+    PairCases_on `p` >>
+    gvs[] >>
+    irule full_entail_super >>
+    first_assum $ irule_at (Pat `lookup _ _ = _`) >>
+    gvs[subst_db_def] >>
+    first_assum $ irule_at (Pos hd) >>
+    first_x_assum irule >>
+    gvs[class_map_to_clk_def]
+  )
+  >- ( (* instance *)
+    Cases_on `p` >>
+    gvs[MEM_MAP,PULL_EXISTS,instance_list_to_ie_def,
+      instance_to_entailment_def,specialises_inst_def] >>
+    irule full_entail_inst >>
+    irule_at Any by_inst_subst >>
+    drule_all inst_map_abs_rel_IMP_well_scoped_inst_map >>
+    drule_then drule $ cj 2 $ iffLR inst_map_abs_rel_def >>
+    rw[inst_abs_rel_def] >>
+    simp[by_inst_def,lookup_inst_map_def,
+      split_ty_cons_tcons_to_type] >>
+    simp[MEM_MAP,PULL_EXISTS,FORALL_PROD] >>
+    rpt strip_tac >>
+    drule_all_then assume_tac $ iffLR well_scoped_inst_map_def >>
+    first_x_assum irule >>
+    gvs[EXISTS_PROD,tcons_to_type_def,subst_db_cons_types,
+      kind_ok_cons_types,EVERY2_MAP,LAMBDA_PROD,EL_GENLIST] >>
+    strip_tac
+    >- (
+      drule_all LIST_REL_MEM_IMP >>
+      simp[EXISTS_PROD]
+    ) >>
+    drule $ iffLR instance_list_kind_ok_def >>
+    disch_then $ drule o SRULE[EVERY_MEM] >>
+    simp[instance_kind_ok_def,entailment_kind_ok_def,
+      instance_to_entailment_def] >>
+    rw[EVERY_MAP,LAMBDA_PROD] >>
+    drule_then drule $ iffLR EVERY_MEM >>
+    rw[] >>
+    simp[] >>
+    irule kind_ok_subst_db >>
+    simp[] >>
+    first_assum $ irule_at (Pat `kind_ok _ _ _ _`) >>
+    rw[]
+    >- (
+      gvs[LIST_REL_EL_EQN] >>
+      last_x_assum drule >>
+      gvs[LLOOKUP_THM]
+    ) >>
+    gvs[LIST_REL_EL_EQN,LLOOKUP_THM]
+  )
 QED
-
-
 
 val _ = export_theory();
